Closing on Blocks + HashSign.
- QC, Votes, Blocks have a sensible definition.
- eliminated most "manual" eqType proofs.
- loosely constrained hashing (different fns for votes & blocks)

Structures/Blocks.v
@@ -4,114 +4,124 @@ Require Import Eqdep.
 From fcsl
 Require Import pred prelude ordtype pcm finmap unionmap heap.
 From LibraChain
-Require Import SeqFacts Chains.
+Require Import SeqFacts Chains HashSign.
+
 Set Implicit Arguments.
 Unset Strict Implicit.
 Unset Printing Implicit Defensive.
 
-Section BlockSource.
+(* We now define VoteData, which is something we know how to hash and sign*)
 
-Variables (Address: finType) (VProof: eqType).
-
-Record BlockSource := mkBS {
-                          author: Address;
-                          signature: VProof;
-                        }.
-
-Definition eq_block_source (b b' : BlockSource) :=
-  match b, b' with
-  | mkBS auth sig, mkBS auth' sig' =>
-    (auth == auth') && (sig == sig')
-  end.
-
-Lemma eq_block_sourceP: Equality.axiom eq_block_source.
-Proof.
-move => bs bs'.
-apply (iffP idP)=> [|->]; last by case bs'=>a' s' //=; rewrite ?eqxx //.
-case bs=> a s; case bs'=> a' s'; [case/andP; move/eqP ->].
-by move/eqP->.
-Qed.
-
-
-Canonical BlockSource_eqMixin :=
-  Eval hnf in EqMixin eq_block_sourceP.
-Canonical BlockSource_eqType :=
-  Eval hnf in EqType BlockSource BlockSource_eqMixin.
-
-End BlockSource.
-
-Section QuorumCert.
-
-Variable Hash: ordType.
-Variable VProof: eqType.
-
-Record QuorumCert := mkQC {
-                      block_hash: Hash;
-                      executed_hash: Hash;
-                      block_round: nat;
-                      parent_block_hash: Hash;
-                      parent_block_round: nat;
-                      grandparent_block_hash: Hash;
-                      grandparent_block_round: nat;
-                      votes: seq VProof;
-                    }.
-
-Definition eq_quorum_cert (qc qc': QuorumCert) :=
-  match qc, qc' with
-  | mkQC bh eh br pbh pbr gpbh gpbr v, mkQC bh' eh' br' pbh' pbr' gpbh' gpbr' v' =>
-    [&& bh == bh', eh == eh', br == br', pbh == pbh', pbr == pbr', gpbh == gpbh', gpbr == gpbr' & v == v']
-  end.
-
-Lemma eq_qcP: Equality.axiom eq_quorum_cert.
- Proof.
-move => qc qc'; apply: (iffP idP) => [| ->].
-- case qc=> bh eh br ph pr gph gpr v;
-  case qc'=> bh' eh' br' ph' pr' gph' gpr' v' /=; do? [case/andP; move/eqP ->]; by move/eqP ->.
-- by case qc'=> bh' eh' br' ph' pr' gph' gpr' v' //=; do? rewrite eqxx.
-Qed.
-
-Canonical QC_eqMixin := Eval hnf in EqMixin eq_qcP.
-Canonical QC_eqType := Eval hnf in EqType QuorumCert QC_eqMixin.
-
-End QuorumCert.
-
+Open Scope sign_scope.
 Section BlockType.
 
-Variables (Hash NodeTime : ordType) (Command VProof : eqType) (Address: finType).
+Variable Hash: ordType.
 
-Record Block :=
-  mkB {
+Record VoteData := mkVD {
+  block_hash: Hash;
+  executed_hash: Hash;
+  block_round: nat;
+  parent_block_hash: Hash;
+  parent_block_round: nat;
+  grandparent_block_hash: Hash;
+  grandparent_block_round: nat;
+}.
+
+(* The VoteMsg assume there's a way to hash and sign VoteData*)
+
+(* TODO: Fix the following line *)
+Import Signable.Exports.
+
+Variables (PublicKey: Type) (Signature: eqType)
+            (HashV: signType VoteData PublicKey Signature).
+
+Definition VD_eqMixin :=
+  Eval hnf in (InjEqMixin (@hash_inj _ HashV)).
+Canonical VD_eqType :=
+  Eval hnf in EqType _ VD_eqMixin.
+
+Variable Address: hashType PublicKey.
+
+Record VoteMsg := mkVM {
+  vote_data: VoteData;
+  vote: (PublicKey * Signature);
+}.
+
+Definition PK_eqMixin :=
+  Eval hnf in InjEqMixin (@hash_inj _ Address).
+Canonical PK_eqType :=
+  Eval hnf in EqType _ PK_eqMixin.
+
+Definition vm2triple (v: VoteMsg) :=
+  let: mkVM vd pks := v in (vd, pks).
+
+Definition triple2vm (triple: VoteData * (PublicKey * Signature)) :=
+  let: (vd, pks) := triple in mkVM vd pks.
+
+Lemma can_vm_triple: ssrfun.cancel vm2triple triple2vm.
+Proof. by move => []. Qed.
+
+Definition vm_eqMixin := CanEqMixin can_vm_triple.
+Canonical vm_eqType := EqType _ vm_eqMixin.
+
+Record QuorumCert := mkQC {
+  voteData: VoteData;
+  votes: seq (PublicKey * Signature);
+}.
+
+Definition qc2votes (qc: QuorumCert) :=
+  let: mkQC vd votes := qc in (vd, votes).
+Definition votes2qc (vs: VoteData * seq (PublicKey * Signature)) :=
+  let: (vd, votes) := vs in mkQC vd votes.
+Lemma can_qc_votes: ssrfun.cancel qc2votes votes2qc.
+Proof. by move => []. Qed.
+
+Definition qc_eqMixin := CanEqMixin can_qc_votes.
+Canonical qc_eqType := EqType _ qc_eqMixin.
+
+(* We can finally define the block type *)
+
+(* The hashability implies the eqType*)
+Variable Command: Type.
+Variable NodeTime: Type.
+
+Record BlockData := mkBD {
     (* Parent's hash pointer *)
-    prevHash : Hash;
+    parent_hash : Hash;
     (* Payload *)
     txs : seq Command;
     (* UnixTime (see liveness) *)
     time: NodeTime;
     round: nat;
     (* Parent's QC information *)
-    proof : QuorumCert Hash VProof;
-    source: BlockSource Address VProof;
-  }.
+    proof : QuorumCert;
+}.
 
-Definition eq_block (b b' : Block) :=
-  match b, b' with
-  | mkB ph txs ti rd pf sc, mkB ph' txs' ti' rd' pf' sc' =>
-    [&& ph == ph', txs == txs', ti == ti', rd == rd', pf == pf' & sc == sc']
-  end.
+Variable hashB: BlockData -> Hash.
+Hypothesis hashB_inj: injective hashB.
 
-Lemma eq_blockP : Equality.axiom eq_block.
-Proof.
-move => b b'.
-apply: (iffP idP) => [|<-].
-- case b => ph txs ti rd pf bs;
-  case b'=> ph' txs' ti' rd' pf' bs'; rewrite /eq_block/=.
-  do? [case /andP; move /eqP ->]; by move /eqP ->.
-- by case b => ph txs ti rd pf bs //=; do? rewrite eqxx.
-Qed.
+Definition Block_hashMixin :=
+  Eval hnf in HashMixin hashB_inj.
 
-Canonical Block_eqMixin :=
-  Eval hnf in EqMixin eq_blockP.
-Canonical Block_eqType :=
-  Eval hnf in EqType Block Block_eqMixin.
+Canonical Block_hashType :=
+  Eval hnf in HashType BlockData Hash Block_hashMixin.
+
+Variable verifB: Hash -> PublicKey -> Signature -> bool.
+
+Definition Block_signMixin :=
+  Eval hnf in SignMixin verifB.
+
+Canonical Block_signType :=
+  Eval hnf in SignType BlockData PublicKey Signature Hash Block_signMixin.
+
+Record BlockType := mkB {
+  block_data: BlockData;
+  block_source: PublicKey * Signature;
+}.
+
+Definition BD_eqMixin :=
+  Eval hnf in (InjEqMixin (@hash_inj _ Block_hashType)).
+Canonical BD_eqType :=
+  Eval hnf in EqType _ BD_eqMixin.
 
 End BlockType.
